isar-ification

DenotSem/DenotAlt.thy
@@ -2,6 +2,10 @@ theory DenotAlt
   imports Denot Deterministic
 begin
 
+definition lamD :: "(ty \<Rightarrow> ty set) \<Rightarrow> ty set" where
+  "lamD G = { f. wf_ty f \<and> fun_pred f \<and> (\<forall> v v'. (v,v') |\<in>| entries f \<longrightarrow>
+                                           (\<exists>v''. v'' \<in> G v \<and> v'' <: v')) }"
+  
 fun D :: "exp \<Rightarrow> ty list \<Rightarrow> ty set" where
   Enat: "D (ENat n) \<rho> = {TNat n}" |
   Evar: "D (EVar k) \<rho> = (if k < length \<rho> then {\<rho>!k} else {})" |
@@ -12,7 +16,11 @@ fun D :: "exp \<Rightarrow> ty list \<Rightarrow> ty set" where
           \<and> v2 \<in> D e2 \<rho> \<and> v1 <: TNat n1 \<and> v2 <: TNat n2 \<and> TNat (f n1 n2) <: v \<and> wf_ty v }" |
   Eif: "D (EIf e1 e2 e3) \<rho> = { v. \<exists> v1 n. v1 \<in> D e1 \<rho> \<and> v1 <: TNat n
          \<and> (n = 0 \<longrightarrow> v \<in> D e3 \<rho>) \<and> (n \<noteq> 0 \<longrightarrow> v \<in> D e2 \<rho>) }"
-
+declare Elam[simp del]
+  
+lemma lambda_lamD[simp]: "D (ELam e) \<rho> = lamD (\<lambda>v. D e (v # \<rho>))"
+  unfolding lamD_def using Elam by blast
+    
 lemma f_lam: "fun_pred f \<Longrightarrow> F f e \<rho> = (\<forall> v v'. (v,v') |\<in>| entries f \<longrightarrow> v' \<in> \<lbrakk>e\<rbrakk> (v#\<rho>))"
   by (induction f) auto
 
@@ -29,39 +37,60 @@ lemma wf_d: "\<lbrakk> wf_env \<rho>; A \<in> D e \<rho> \<rbrakk> \<Longrightar
   apply (induction e arbitrary: \<rho> A)
        apply simp apply (case_tac "x < length \<rho>") apply force apply force
       apply force
-     apply force
+     using lamD_def apply force
   using D.simps(4) apply blast
    apply (smt D.simps(5) mem_Collect_eq)
   by (smt D.simps(6) mem_Collect_eq)
     
 theorem d_e: "wf_env \<rho> \<Longrightarrow> \<lbrakk>e\<rbrakk>\<rho> = {B. \<exists>A. A \<in> D e \<rho> \<and> A <: B \<and> wf_ty B }"  
-  apply (induction e arbitrary: \<rho>)
-       apply force
-      apply force
-    -- "lambda" 
-     apply simp apply (rule Collect_cong) apply (rule iffI) 
-      apply clarify
-      apply (rule_tac x=f in exI) apply simp apply (rule conjI)
-  using f_fun_pred apply blast
-      apply clarify    
-      apply (subgoal_tac "wf_ty v \<and> wf_ty v'") prefer 2 apply (rule wf_entries) apply blast apply blast
-      apply (subgoal_tac "wf_env (v#\<rho>)") prefer 2 apply (rule extend_wf_env) apply blast apply blast
-      apply (subgoal_tac "\<lbrakk>e\<rbrakk>(v#\<rho>) = {B. \<exists>A. A \<in> D e (v#\<rho>) \<and> A <: B \<and> wf_ty B}")
-       prefer 2 apply blast
-      apply (subgoal_tac "v' \<in> \<lbrakk>e\<rbrakk>(v#\<rho>)") prefer 2 using f_lam f_fun_pred apply meson 
-      apply (subgoal_tac "\<exists>A. A \<in> D e (v # \<rho>) \<and> A <: v' \<and> wf_ty v'") prefer 2 apply blast
-      apply clarify
-      apply blast
-     apply clarify 
-     apply (subgoal_tac "F A e \<rho> = (\<forall> v v'. (v,v') |\<in>| entries A \<longrightarrow> v' \<in> \<lbrakk>e\<rbrakk> (v#\<rho>))") prefer 2
-      apply (rule f_lam) apply blast
-     apply (subgoal_tac "F A e \<rho>")       
-      apply (rule subsumption_fun) apply assumption apply assumption apply assumption
-        apply assumption apply assumption apply clarify apply (meson subsumption)
-     apply (subgoal_tac "\<forall> v v'. (v,v') |\<in>| entries A \<longrightarrow> v' \<in> \<lbrakk>e\<rbrakk> (v#\<rho>)") apply blast
-     apply (metis (no_types, lifting) extend_wf_env mem_Collect_eq wf_entries)
-    -- "app"
-    apply simp apply (rule Collect_cong) apply (rule iffI) 
+proof (induction e arbitrary: \<rho>)
+  case (EVar x)
+  then show ?case by auto
+next
+  case (ENat x)
+  then show ?case by auto
+next
+  case (ELam e)
+  { fix f assume wf_f: "wf_ty f" and f_f: "F f e \<rho>"
+    have fun_f: "fun_pred f" using f_f f_fun_pred by blast
+    have "f \<in> lamD (\<lambda>v. D e (v # \<rho>))" using wf_f fun_f apply (simp add: lamD_def) apply clarify
+    proof -
+      fix v v' assume vv_f: "(v, v') |\<in>| entries f"
+      have 1: "v' \<in> \<lbrakk>e\<rbrakk> (v#\<rho>)" using f_f fun_f f_lam[of f] vv_f by blast
+      have wf_vr: "wf_env (v#\<rho>)"
+        using vv_f wf_entries[of f v v'] extend_wf_env[of \<rho> v] wf_f ELam.prems by blast
+      have "\<lbrakk>e\<rbrakk>v # \<rho> = {B. \<exists>A. A \<in> D e (v # \<rho>) \<and> A <: B \<and> wf_ty B}" 
+        using ELam.IH[of "v#\<rho>"] wf_vr by blast
+      then show "\<exists>v''. v'' \<in> D e (v # \<rho>) \<and> v'' <: v' " using 1 by auto
+    qed        
+    then have "\<exists>A. A \<in> lamD (\<lambda>v. D e (v # \<rho>)) \<and> A <: f \<and> wf_ty f" using wf_f by auto
+  } moreover { fix f assume "\<exists>A. A \<in> lamD (\<lambda>v. D e (v # \<rho>)) \<and> A <: f \<and> wf_ty f"
+    then obtain A where A_D: "A \<in> lamD (\<lambda>v. D e (v # \<rho>))" and A_f: "A <: f" and wf_f: "wf_ty f"
+      by blast
+    have fun_A: "fun_pred A" using A_D by (simp add: lamD_def) 
+    have wf_A: "wf_ty A" using A_D by (simp add: lamD_def) 
+    have "\<forall> v v'. (v,v') |\<in>| entries A \<longrightarrow> v' \<in> \<lbrakk>e\<rbrakk> (v#\<rho>)"
+    proof clarify
+      fix v v' assume vv_A: "(v,v') |\<in>| entries A"
+      have wf_vr: "wf_env (v#\<rho>)"
+        using vv_A wf_entries[of A v v'] extend_wf_env[of \<rho> v] wf_A ELam.prems by blast
+      have "\<lbrakk>e\<rbrakk>v # \<rho> = {B. \<exists>A. A \<in> D e (v # \<rho>) \<and> A <: B \<and> wf_ty B}" 
+        using ELam.IH[of "v#\<rho>"] wf_vr by blast
+      
+      then 
+      show "v' \<in> \<lbrakk>e\<rbrakk>(v#\<rho>)" 
+        by (smt A_D lamD_def mem_Collect_eq vv_A wf_entries)
+    qed      
+    then have F_A: "F A e \<rho>" using f_lam fun_A by blast
+    then have F_f: "F f e \<rho>" using subsumption_fun[of A e \<rho> f] A_f
+        subsumption A_D ELam.prems lamD_def wf_f by blast      
+    then have "wf_ty f \<and> F f e \<rho>" using wf_f by blast }
+  ultimately show ?case apply simp
+    apply (rule Collect_cong) apply (rule iffI) apply blast apply blast done
+next
+  case (EApp e1 e2)
+  then show ?case 
+      apply simp apply (rule Collect_cong) apply (rule iffI) 
      apply clarify apply (rule_tac x=v' in exI) apply (rule conjI)
       apply (rule_tac x=A in exI) apply (rule conjI) apply assumption
       apply (rule_tac x=Aa in exI) apply (rule conjI) apply assumption
@@ -75,16 +104,22 @@ theorem d_e: "wf_env \<rho> \<Longrightarrow> \<lbrakk>e\<rbrakk>\<rho> = {B. \<
       apply assumption apply assumption apply (rule conjI) 
      apply (subgoal_tac "v \<rightarrow> A <: v \<rightarrow> v'") prefer 2 apply blast
      apply (meson sub_trans) apply assumption 
-    -- "prim"
-   apply simp apply (rule Collect_cong) apply (rule iffI)
+      done
+next
+  case (EPrim x1a e1 e2)
+  then show ?case 
+    apply simp apply (rule Collect_cong) apply (rule iffI)
     apply (meson sub_refl sub_trans)
-   apply (meson sub_refl sub_trans wf_d)
-    -- "if"
-  apply simp apply (rule Collect_cong) apply (rule iffI)
+   apply (meson sub_refl sub_trans wf_d) done
+next
+  case (EIf e1 e2 e3)
+  then show ?case 
+    apply simp apply (rule Collect_cong) apply (rule iffI)
    apply clarify
    apply (case_tac n) apply simp apply clarify
     apply (meson less_numeral_extra(3) sub_trans)
    apply (meson Suc_neq_Zero sub_trans zero_less_Suc)
   by blast
+qed
 
 end
